\section{Reglas de evaluación de tail.}
\label{apendice:evaluacion_tail}

\begin{figure}[p]
\caption{Reglas de evaluación de tail.}
\label{fig:evtail}

\bigskip
\bigskip

\inference[E-AssigRed:]{t -> t'}{x \<:=> t -> x \<:=> t'}

\bigskip

\inference[E-Assig:]
{x \<:=> v}
{\begin{array}{@{}c@{}}
\Gamma |- x \<:=> v \\
x\<:=>v -> v
\end{array}}

\bigskip

\inference[E-Var:]{\Gamma |- x \<:=> v}{x -> v}

\bigskip

\inference[E-TypeDec:]{}{t:\tau -> t}

\bigskip

\inference[E-Typeof:]{\Gamma |- t : \tau}{\<typeof> t -> string(\tau)}

\bigskip

\inference[E-FuncSintSug:]{}{f(x) := t -> f := \<lambda> x.t}

\bigskip

\inference[E-App:]{}{\<lambda> x . t (v) -> [x |-> v]t}

\bigskip

\inference[E-AppParameterRed:]{t -> t'}{\<lambda> x . \overline{t} (t) -> \<lambda> x . \overline{t} (t')}

\bigskip

\inference[E-AppRed:]{t_1 -> t_1'}{t_1(t_2) -> t_1'(t_2)}

\bigskip

\inference[E-If:]{}{\<if> True \<then> t_1 \<else> t_2 -> t_1}

\bigskip

\inference[E-Else:]{}{\<if> False \<then> t_1 \<else> t_2 -> t_2}

\bigskip

\inference[E-IfRed:]{t_1 -> t_1'}{\<if> t_1 \<then> t_2 \<else> t_3 -> \<if> t_1' \<then> t_2\ \<else> t_3}

\bigskip

\inference[E-Seq:]{t_1 -> t_1'}{t_1 \<;> t_2 -> t_1' \<;> t_2}

\bigskip

\inference[E-SeqNext:]{}{v \<;> t -> t}

\bigskip

\inference[E-ParRed:]{t -> t'}{(t) -> (t')}

\bigskip

\inference[E-Par:]{}{(v) -> v}

\bigskip

\inference[E-BlockRed:]
{t -> t'}
{
\Gamma' := \Gamma, \\
BeginBlock\ t\ EndBlock ->_{\Gamma'} BeginBlock\ t'\ EndBlock
}

\bigskip

\inference[E-Block:]{}{BeginBlock\ v\ EndBlock -> v}

\end{figure}


\begin{figure}[p]

\bigskip
\bigskip

\inference[E-String:]{}{``v^s \{v\} t^s" -> ``v^s" + string(v) + ``t^s"}

\bigskip

\inference[E-StringRed:]{t -> t'}{``v^s \{t\} t^s" -> ``v^s \{t'\} t^s"}

\inference[E-SubTypeTrue:]{\tau_1 ~< \tau_2}{\tau_1 \<<:> \tau_2 -> True}

\bigskip

\inference[E-SubTypeFalse:]{\tau_1 \ \widetilde{\nleq}\ \tau_2}{\tau_1 \<<:> \tau_2 -> False}

\bigskip

\inference[E-VariantDec:]{}{
\begin{array}{@{}c@{}}
\<variant> V \<::> C_1(l_{1 1} : \tau_{11}, ..., l_{1r_1} : \tau_{1r_1}) \mid ... \mid C_n(l_{n 1} : \tau_{n 1}, ..., l_{nr_n} : \tau_{nr_n}) -> \\
-> <{V::C_i(l_{ij} : \tau_{ij}}^{j \in 1...r_i})^{i \in 1...n}> \\
\Gamma |- V := {V::C_i({l_{ij} : \tau_{ij}}^{j \in 1...r_i})}^{i \in 1...n}
\end{array}}

\bigskip

\inference[E-VariantConstruct:]{\Gamma |- V := {V::C_i(l_{ij} : \tau_{ij}}^{j \in 1...r_i})^{i \in 1...n}}{
\begin{array}{@{}c@{}}
\Gamma |- V::C_i := \lambda x_1, ..., x_{r_i}.V::C_i(l_{ij} : \tau_{ij}^{j \in 1 ... r_i})^{i \in 1...n}
\end{array}}

\bigskip

\inference[E-ProjectionVariant:]{
\<variant> {V::C_i(x_{ij} : \tau_{ij}}^{j \in 1...r_i})^{i \in 1...n} \in \Gamma
}{
V::C_i(t_{i1}, ..., t_{in}).x_{ik} -> t_{ik}
}

\bigskip

\inference[E-DotRed:]{t_1 -> t'_1}{t_1.x -> t'_1.x}

\bigskip

\inference[E-MethodSintSug:]{}{t_1.t_2(t_3) -> t_2(t_1, t_3)}

\bigskip

\inference[E-MatchRed:]{t_0 -> t'_0}{
\begin{array}{@{}c@{}}
\<match> t_0 \<with>\ t_{1i}\ \mathligsoff -> \mathligson\ t_{2i} -> \\
->\ \<match> t'_0 \<with>\ t_{1i}\ \mathligsoff -> \mathligson\ t_{2i}
\end{array}}

\bigskip

\inference[E-MatchPatternRed:]{t_{1i} -> t'_{1i}}{
\begin{array}{@{}c@{}}
\<match> v \<with>\ t_{1i}\ \mathligsoff -> \mathligson\ t_{2i} -> \\
->\ \<match> v \<with>\ t'_{1i}\ \mathligsoff -> \mathligson\ t_{2i}
\end{array}}

\bigskip

\inference[E-MatchEqual:]{v_i=v_0\ y\ v_j \neq v_0\ \forall\ 0 < j < i}{
\begin{array}{@{}c@{}}
\<match>\ v_0 \<with> v_i\ \mathligsoff -> \mathligson\ t_i -> t_i
\end{array}}

\bigskip

\inference[E-MatchAny:]{}{
\begin{array}{@{}c@{}}
\<match>\ v \<with> \_\ \mathligsoff -> \mathligson\ t_i -> t_i
\end{array}}

\bigskip

\inference[E-MatchVariant:]{}{
\begin{array}{@{}c@{}}
\<match>\ V::C_i(v_1, ..., v_n) \<with>\\
V::C_i(x_1, ..., x_n)\ \mathligsoff -> \mathligson\ t_i -> [x_i |-> v_i]t_i
\end{array}}

\bigskip

\end{figure}


\begin{figure}[p]

\bigskip
\bigskip

\inference[E-Tuple:]
{t_j -> t'_j}
{v_i^{i \in 1...j-1}, t_j, t_k^{k \in j+1...n} -> v_i^{i \in 1...j-1}, t'_j, t_k^{k \in j+1...n}}

\bigskip

\inference[E-AssigTuple:]
{}
{x_i^{i \in 1...n} := t_i^{i \in 1...n} -> x_i := t_i\ i \in 1...n}

\bigskip

\inference[E-MatchTuple:]{}
{\<match>\ v_i^{i \in 1...n} \<with>\ x_i^{i \in 1...n} \mathligsoff -> \mathligson\ t ->
[x_i |-> v_i]t}

\bigskip


\inference[E-List:]
{t_j -> t'_j}
{<v_i^{i \in 1...j-1}\ t_j\ t_k^{k \in j+1...n}> -> <v_i^{i \in 1...j-1}\ t'_j\ t_k^{k \in j+1...n}>}

\bigskip

\inference[E-MatchList:]{}
{\<match>\ <v_i^{i \in 1...n}>\ \<with>\ <x \mid \overline{x}> \mathligsoff -> \mathligson\ t ->
[x |-> v_1, \overline{x} |-> <v_i^{i \in 2...n}>]t}

\bigskip

\inference[E-Vector:]
{t_j -> t'_j}
{[v_i^{i \in 1...j-1}\ t_j\ t_k^{k \in j+1...n}] -> [v_i^{i \in 1...j-1}\ t'_j\ t_k^{k \in j+1...n}]}

\bigskip

\inference[E-Matrix:]
{t_{rk} -> t'_{rk}}
{[v_{ij}^{\stackrel{i \in 1...r-1}{j \in 1...m}} \mid
v_{rj}^{j \in 1...k-1}\ t_{rk}\ t_{rj}^{j \in k+1...m} \mid
v_{ij}^{\stackrel{i \in r+1...n}{j \in 1...m}}] ->
[v_{ij}^{\stackrel{i \in 1...r-1}{j \in 1...m}} \mid
v_{rj}^{j \in 1...k-1}\ t'_{rk}\ t_{rj}^{j \in k+1...m} \mid
v_{ij}^{\stackrel{i \in r+1...n}{j \in 1...m}}]}

\bigskip

\inference[E-DictKey:]
{t_j -> t'_j}
{{v_i => \overline{v}_i}^{i \in 1...j-1}, t_j => \overline{t}_j, {t_k => \overline{t}_k}^{k \in j+1...n} -> 
{v_i => \overline{v}_i}^{i \in 1...j-1}, t'_j => \overline{t}_j, {t_k => \overline{t}_k}^{k \in j+1...n}}

\bigskip

\inference[E-DictValue:]
{\overline{t}_j -> \overline{t'}_j}
{{v_i => \overline{v}_i}^{i \in 1...j-1}, v_j => \overline{t}_j, {t_k => \overline{t}_k}^{k \in j+1...n} -> 
{v_i => \overline{v}_i}^{i \in 1...j-1}, v_j => \overline{t'}_j, {t_k => \overline{t}_k}^{k \in j+1...n}}
\end{figure}
